Lp2lc/Active/STLC PHOAS/Example.lean
@@ -1,0 +1,11 @@
+import «Lp2lc».Active.STLC.Proof
+
+namespace Lp2lc.Active.STLC
+
+namespace Example
+
+-- contains verified examples and test cases of things in Def
+
+-- All docstrings use short (under 5 lines) of Scala code as demonstrations.
+
+end Example
